floyd/loadstore_lemmas.v
@@ -1,0 +1,1117 @@
+Require Import floyd.base.
+Require Import floyd.client_lemmas.
+Require Import floyd.field_mapsto.
+Require Import floyd.assert_lemmas.
+
+Local Open Scope logic.
+
+Lemma mapsto_force_ptr: forall sh t v v', 
+  mapsto sh t (force_ptr v) v' = mapsto sh t v v'.
+Proof.
+intros.
+destruct v; simpl; auto.
+Qed.
+
+Lemma isptr_force_ptr: forall v, isptr v -> force_ptr v = v.
+Proof. intros. destruct v; inv H; auto. Qed.
+
+Lemma local_andp_lemma:
+  forall P Q, P |-- local Q -> P = local Q && P.
+Proof.
+intros.
+apply pred_ext.
+apply andp_right; auto.
+apply andp_left2; auto.
+Qed.
+
+Lemma semax_load'':
+  forall Espec (Delta : tycontext) (sh : Share.t) (id : positive) (n: nat)
+         P Q R (e1 : expr) t1 i2 (v1 v2 : environ -> val),
+   typeof e1 = Tpointer t1 noattr ->
+   (temp_types Delta) ! id = Some (t1,i2) ->
+   type_is_volatile t1 = false ->
+   classify_cast t1 t1 = cast_case_neutral ->
+    PROPx P (LOCALx (tc_environ Delta :: Q) (SEPx R)) |-- local (tc_expr Delta e1) ->
+    PROPx P (LOCALx (tc_environ Delta :: Q) (SEPx R)) |-- local (`eq v1 (eval_expr e1)) ->
+    nth_error R n = Some (`(mapsto sh t1) v1 v2) ->
+ @semax Espec Delta  
+    (|> PROPx P (LOCALx Q (SEPx R)))
+    (Sset id (Ederef e1 t1))
+    (normal_ret_assert
+       (EX old: val, 
+        PROPx P (LOCALx (`eq (eval_id id) (subst id (`old) v2) ::
+                         map (subst id (`old)) Q)
+                (SEPx 
+                  (map (subst id (`old))
+                    (replace_nth n R (`(mapsto sh t1) (eval_expr e1) v2))))))).
+Proof.
+ intros. rename H2 into CLASSIFY.
+ eapply semax_pre_post;
+  [ | |  apply (semax_load Delta sh id (PROPx P (LOCALx Q (SEPx (replace_nth n R emp)))) (Ederef e1 t1)
+   v2)]; auto.
+assert (PROPx P (LOCALx (tc_environ Delta :: Q) (SEPx R)) |-- local (`isptr (eval_expr e1))).
+ {clear - H4 H5.
+  rewrite (local_andp_lemma _ _ H4).
+  clear H4.
+  unfold_lift.
+  change SEPx with SEPx'; unfold PROPx,LOCALx,SEPx',local,lift1; intro rho; simpl in *.
+  apply derives_extract_prop; intro. unfold_lift in H. rewrite <- H. clear e1 H.
+  apply andp_left2. apply andp_left2.
+  unfold_lift in H5.
+  revert R H5; induction n; destruct R; intros; inv H5; simpl in *; auto.
+  rewrite mapsto_isptr. normalize.
+  apply derives_trans with (TT * (!!isptr (v1 rho) && TT)).
+  apply sepcon_derives; auto. rewrite andp_TT. auto.
+  normalize.
+ }
+eapply derives_trans; [apply andp_derives; [ apply now_later | apply derives_refl] | ].
+rewrite <- later_andp.
+apply later_derives.
+rewrite insert_local.
+repeat apply andp_right.
+rewrite (local_andp_lemma _ _ H4).
+rewrite (local_andp_lemma _ _ H3).
+rewrite (local_andp_lemma _ _ H2).
+repeat rewrite <- andp_assoc. apply andp_left1.
+intro rho; unfold local, lift1.
+clear - H H1; simpl; normalize.
+unfold tc_expr, tc_lvalue in *; simpl in *.
+rewrite H1. rewrite H. simpl.
+repeat rewrite tc_andp_TT2.
+rewrite denote_tc_assert_andp.
+simpl.
+split; auto.
+unfold tc_temp_id_load. rewrite H0.
+intro rho.
+simpl.
+apply prop_right.
+do 2 eexists; split; try reflexivity.
+unfold allowedValCast; simpl. rewrite CLASSIFY.
+destruct t1; simpl; auto.
+rewrite (local_andp_lemma _ _ H4).
+simpl typeof; simpl eval_lvalue.
+apply derives_trans with 
+ (local (`eq v1 (eval_expr e1)) && (`(mapsto sh t1) v1 v2 *
+       PROPx P (LOCALx Q (SEPx (replace_nth n R emp))))).
+rewrite <- insert_local.
+apply andp_derives; auto.
+apply andp_left2.
+clear - H5.
+change SEPx with SEPx'; unfold PROPx,LOCALx,SEPx',local,lift1; intro rho; simpl.
+normalize.
+clear - H5; revert R H5; induction n; destruct R; simpl; intros; inv H5.
+rewrite emp_sepcon; apply sepcon_derives; auto.
+rewrite <- sepcon_assoc.
+rewrite (sepcon_comm (mapsto _ _ _ _)).
+rewrite sepcon_assoc.
+apply sepcon_derives; auto.
+intro rho; unfold_lift.
+unfold local, lift1; simpl.
+normalize.
+rewrite mapsto_force_ptr.
+rewrite H6; auto.
+
+intros ek vl rho.
+unfold normal_ret_assert.
+normalize. 
+apply exp_right with old.
+normalize. simpl typeof; unfold eval_lvalue; fold eval_expr.
+autorewrite with subst.
+change SEPx with SEPx'; unfold PROPx,LOCALx,SEPx',local,lift1.
+normalize.
+rewrite mapsto_force_ptr.
+clear - H5.
+revert R H5; induction n; destruct R; simpl; intros; auto; inv H5.
+apply sepcon_derives; simpl; auto.
+rewrite closed_wrt_subst by (auto with closed).
+rewrite emp_sepcon; auto.
+specialize (IHn _ H0).
+rewrite <- sepcon_assoc.
+rewrite (sepcon_comm (mapsto _ _ _ _)).
+rewrite sepcon_assoc.
+apply sepcon_derives; auto.
+Qed.
+
+Lemma semax_store'':
+forall Espec (Delta: tycontext) sh t1 n P Q R e1 v1 e2
+    (WS: writable_share sh)
+    (NONVOL: type_is_volatile t1 = false)
+    (TC: typecheck_store (Ederef e1 t1)),
+    typeof e1 = Tpointer t1 noattr ->
+    nth_error R n = Some (`(mapsto_ sh t1) v1) ->
+    PROPx P (LOCALx (tc_environ Delta :: Q) (SEP (TT))) |-- local (`eq v1 (eval_expr e1)) ->
+    PROPx P (LOCALx (tc_environ Delta :: Q) (SEPx R)) |-- local (tc_expr Delta e1) ->
+    PROPx P (LOCALx (tc_environ Delta :: Q) (SEPx R)) |-- local (tc_expr Delta (Ecast e2 t1)) ->
+    @semax Espec Delta 
+       (|> PROPx P (LOCALx Q (SEPx R)))
+       (Sassign (Ederef e1 t1) e2) 
+       (normal_ret_assert
+          (PROPx P (LOCALx Q
+              (SEPx (replace_nth n R
+                    (`(mapsto sh t1) v1 (`(eval_cast (typeof e2) t1) (eval_expr e2)))))))).
+Proof.
+intros.
+pose proof semax_store.
+unfold_lift; unfold_lift in H0.
+eapply semax_pre_post; [ | | eapply (H4 Delta (Ederef e1 t1) e2 sh)]; try eassumption.
+instantiate (1:=(PROPx P (LOCALx Q (SEPx (replace_nth n R emp))))).
+assert (H1': PROPx P (LOCALx (tc_environ Delta :: Q) (SEPx R)) |-- local (`eq v1 (eval_expr e1))).
+ {  eapply derives_trans; [ | apply H1].
+  apply andp_derives; auto. apply andp_derives; auto. change SEPx with SEPx'; unfold SEPx'.
+  unfold fold_right at 2. rewrite sepcon_emp. apply TT_right.
+ }
+assert (PROPx P (LOCALx (tc_environ Delta :: Q) (SEPx R)) |-- local (`isptr (eval_expr e1))).
+  {clear - H1' H0. rename H1' into H4; rename H0 into H5.
+   rewrite (local_andp_lemma _ _ H4).
+   clear H4.
+   unfold_lift.
+   change SEPx with SEPx'; unfold PROPx,LOCALx,SEPx',local,lift1; intro rho; simpl in *.
+   apply derives_extract_prop; intro. unfold_lift in H. rewrite <- H. clear e1 H.
+   apply andp_left2. apply andp_left2.
+   unfold_lift in H5.
+   revert R H5; induction n; destruct R; intros; inv H5; simpl in *; auto.
+   rewrite mapsto__isptr. normalize.
+   apply derives_trans with (TT * (!!isptr (v1 rho) && TT)).
+   apply sepcon_derives; auto. rewrite andp_TT. auto.
+   normalize.
+  }
+eapply derives_trans; [apply andp_derives; [ apply now_later | apply derives_refl] | ].
+rewrite <- later_andp.
+apply later_derives.
+rewrite insert_local.
+rewrite (local_andp_lemma _ _ H1').
+rewrite (local_andp_lemma _ _ H2).
+rewrite (local_andp_lemma _ _ H3).
+rewrite (local_andp_lemma _ _ H5).
+change SEPx with SEPx'.
+intro rho; unfold PROPx, LOCALx, SEPx', local, lift1,lift2.
+simpl.
+unfold_lift.
+repeat (apply derives_extract_prop; intro).
+destruct H11.
+unfold tc_lvalue. simpl typecheck_lvalue.
+repeat rewrite denote_tc_assert_andp.
+rewrite H; simpl.
+
+rewrite isptr_force_ptr by auto.
+repeat apply andp_right; try apply prop_right; auto.
+repeat split; auto.
+rewrite NONVOL; hnf; unfold_lift; hnf; auto.
+rewrite prop_true_andp by auto.
+rewrite prop_true_andp by auto.
+rewrite <- H6.
+clear - H0.
+revert R H0; induction n; destruct R; simpl; intros; inv H0; auto.
+rewrite emp_sepcon; auto.
+rewrite <- sepcon_assoc.
+rewrite (sepcon_comm (mapsto_ _ _ _)).
+rewrite sepcon_assoc.
+apply sepcon_derives; auto.
+
+intros ek vl rho; unfold normal_ret_assert, local,lift1; unfold_lift; simpl. unfold_lift.
+match goal with |- ?A |-- _ => apply derives_trans with (local (`eq v1 (eval_expr e1)) rho && A) end.
+apply andp_right.
+eapply derives_trans; [ | apply H1].
+rewrite <- insert_local.
+simpl.
+apply andp_derives.
+apply prop_derives.
+clear. 
+unfold tc_environ, exit_tycon. destruct ek; auto.
+repeat (apply derives_extract_prop; intro).
+subst.
+change SEPx with SEPx'; unfold PROPx,LOCALx,SEPx',local,lift1; simpl.
+clear. induction R; normalize.
+repeat (apply derives_extract_prop; intro).
+repeat (rewrite prop_true_andp by auto).
+auto.
+repeat (apply derives_extract_prop; intro).
+unfold_lift in H5. rewrite <- H5.
+repeat (rewrite prop_true_andp by auto).
+normalize.
+rewrite mapsto_force_ptr.
+clear - H0. revert R H0; induction n; destruct R; simpl; intros; inv H0.
+rewrite emp_sepcon; auto.
+rewrite <- sepcon_assoc.
+rewrite (sepcon_comm (mapsto _ _ _ _)).
+rewrite sepcon_assoc.
+apply sepcon_derives; auto.
+Qed.
+
+
+Lemma semax_load_field:
+forall Espec (Delta: tycontext) sh id t1 fld P e1 v2 t2 i2 sid fields ,
+    typeof e1 = Tstruct sid fields noattr ->
+    (temp_types Delta) ! id = Some (t2,i2) ->
+   t1 = typeof e1 ->
+   t2 = type_of_field
+             (unroll_composite_fields sid (Tstruct sid fields noattr) fields) fld ->
+   Cop.classify_cast t2 t2 = Cop.cast_case_neutral ->
+    @semax Espec Delta 
+       (|> (local (tc_lvalue Delta e1) &&
+          (`(field_mapsto sh t1 fld) (eval_lvalue e1) v2 * P)))
+       (Sset id (Efield e1 fld t2))
+       (normal_ret_assert (
+         EX old:val, local (`eq (eval_id id) (subst id (`old) v2)) &&
+                  (subst id (`old) 
+                    (`(field_mapsto sh t1 fld) (eval_lvalue e1) v2 * P)))).
+Proof.
+Transparent field_mapsto.
+pose proof I.
+pose proof I.
+intros. rename H5 into CLASSIFY.
+rename H3 into TC0; rename H4 into TC2.
+subst t1.
+rename H2 into TE1.
+apply (semax_pre_post
+            (|>(local (tc_lvalue Delta (Efield e1 fld t2)) &&
+                 local (tc_temp_id_load id (typeof (Efield e1 fld t2)) Delta v2) && 
+               (`(mapsto sh t2) (eval_lvalue (Efield e1 fld t2)) v2 * 
+                        ( !!(type_is_volatile t2 = false) &&  P))))
+            (normal_ret_assert 
+              (EX old:val, local (`eq (eval_id id) (subst id (`old) v2)) &&
+              (subst id (`old) (`(mapsto sh t2) (eval_lvalue (Efield e1 fld t2)) v2  * 
+                (!!(type_is_volatile t2 = false) && P))))));
+  [ | | apply semax_load].
+
+(* PRECONDITION *)
+intro rho.
+unfold tc_temp_id_load, local,lift1.  unfold_lift.
+simpl.
+apply derives_extract_prop; intro.
+apply later_derives.
+apply derives_extract_prop; intro.
+unfold field_mapsto; unfold_lift. 
+case_eq (eval_lvalue e1 rho); intros; 
+ try (rewrite FF_sepcon; apply FF_left).
+rewrite H1.
+rewrite field_offset_unroll. rewrite <- TC2.
+case_eq (field_offset fld fields); intros; 
+ try (rewrite FF_sepcon; apply FF_left).
+case_eq (access_mode t2); intros;
+ try (rewrite FF_sepcon; apply FF_left).
+normalize.
+repeat apply andp_right; try apply prop_right.
+unfold tc_lvalue. 
+unfold typecheck_lvalue; fold typecheck_lvalue. rewrite H1.
+rewrite H8; simpl tc_bool.
+rewrite H5. repeat rewrite tc_andp_TT2.
+apply H3.
+exists t2; exists i2; split; auto.
+unfold allowedValCast. rewrite CLASSIFY.
+destruct t2; simpl; auto. auto.
+unfold mapsto.
+normalize.
+unfold umapsto.
+rewrite H6.
+unfold eval_field. rewrite H5.
+simpl. apply sepcon_derives; auto. apply orp_right1. auto.
+
+(* POSTCONDITION *)
+intros ek vl.
+apply andp_left2.
+intro rho. apply normal_ret_assert_derives.
+unfold local, lift1; unfold_lift; simpl.
+apply exp_derives. intro old.
+apply andp_derives; auto.
+unfold subst. unfold_lift.
+unfold mapsto, field_mapsto, umapsto.
+rewrite H1. rewrite <- TC2.
+normalize.
+case_eq (access_mode t2); intros; 
+ try (rewrite FF_sepcon; apply FF_left).
+simpl eval_field. unfold always.
+rewrite field_offset_unroll. unfold offset_val.
+destruct (field_offset fld fields);  try (rewrite FF_sepcon; apply FF_left).
+destruct (eval_lvalue e1 (env_set rho id old)); try (rewrite FF_sepcon; apply FF_left).
+normalize.
+apply sepcon_derives; auto.
+apply orp_left; auto.
+normalize. rewrite H5 in H2; inv H2.
+Qed.
+
+
+Lemma semax_store_field: 
+forall Espec (Delta: tycontext) sh e1 fld P t2 e2 sid fields ,
+    writable_share sh ->
+    typeof e1 = Tstruct sid fields noattr ->
+    t2 = type_of_field
+             (unroll_composite_fields sid (Tstruct sid fields noattr) fields) fld ->
+    typecheck_store (Efield e1 fld t2) ->
+   @semax Espec Delta 
+       (|> (local (tc_lvalue Delta e1) && local (tc_expr Delta (Ecast e2 t2)) &&
+          (`(field_mapsto_ sh (typeof e1) fld) (eval_lvalue e1) * P)))
+       (Sassign (Efield e1 fld t2) e2) 
+       (normal_ret_assert 
+          (`(field_mapsto sh (typeof e1) fld) (eval_lvalue e1) 
+                  (`(eval_cast (typeof e2) t2) (eval_expr e2)) * P)).
+Proof.
+Transparent field_mapsto.
+pose proof I. intros until fields. intro WS.
+intros.
+rename H0 into TE1.
+rename H2 into TCS.
+unfold field_mapsto_.
+
+apply semax_pre0 with
+ (EX v2: val,
+   ((|>(local (tc_lvalue Delta e1) && local (tc_expr Delta (Ecast e2 t2)) &&
+      (lift1(fun v1 : val =>
+         match v1 with
+         | Vundef => FF
+         | Vint _ => FF
+         | Vfloat _ => FF
+         | Vptr l ofs =>
+             match typeof e1 with
+             | Tstruct id fList _ =>
+                 match
+                   field_offset fld
+                     (unroll_composite_fields id (typeof e1) fList)
+                 with
+                 | Errors.OK delta =>
+                     match
+                       access_mode
+                         (type_of_field
+                            (unroll_composite_fields id (typeof e1) fList)
+                            fld)
+                     with
+                     | By_value ch =>
+                         !!(type_is_volatile
+                              (type_of_field
+                                 (unroll_composite_fields id (typeof e1)
+                                    fList) fld) = false) &&
+                         (address_mapsto ch v2 (Share.unrel Share.Lsh sh)
+                            (Share.unrel Share.Rsh sh)
+                            (l, Int.unsigned (Int.add ofs (Int.repr delta))))
+                     | _ => FF
+                     end
+                 | _ => FF
+                 end
+             | _ => FF
+             end
+         end) (eval_lvalue e1) * P))))).
+rewrite <- later_exp' by apply Vundef.
+apply later_derives.
+rewrite <- exp_andp2.
+apply andp_derives; auto.
+unfold lift1; intro rho; unfold_lift.
+simpl sepcon. cbv beta.
+case_eq (eval_lvalue e1 rho); intros; try rewrite FF_sepcon; try apply FF_left.
+destruct (typeof e1);  try rewrite FF_sepcon; try apply FF_left.
+destruct (field_offset fld (unroll_composite_fields i0 (Tstruct i0 f a) f));
+   try (rewrite FF_sepcon; apply FF_left).
+destruct ( access_mode
+    (type_of_field (unroll_composite_fields i0 (Tstruct i0 f a) f) fld));
+   try (rewrite FF_sepcon; apply FF_left).
+normalize.
+apply exp_right with v2. rewrite H0. normalize.
+apply extract_exists_pre; intro v0.
+
+pose proof (semax_store Delta (Efield e1 fld t2) e2 sh 
+               (local (`(tc_val t2) (`(eval_cast (typeof e2) t2) (eval_expr e2))) &&
+                 !! (type_is_volatile t2 = false) &&   P)).
+simpl typeof in H0. 
+eapply semax_pre_post ; [ | | apply H0; auto]; clear H0.
+match goal with |- (?A && |> ?B |-- |> ?C) =>
+  apply derives_trans with (|> (A && B));
+    [rewrite (later_andp A B); apply andp_derives; auto; apply now_later 
+    | apply later_derives]
+end.
+intro rho; unfold lift1; unfold_lift.
+ simpl andp; simpl sepcon. cbv beta.
+rewrite TE1.
+normalize.
+unfold mapsto_, umapsto.
+case_eq (eval_lvalue e1 rho); intros; try (rewrite FF_sepcon; apply FF_left).
+case_eq (field_offset fld
+    (unroll_composite_fields sid (Tstruct sid fields noattr) fields)); intros; try (rewrite FF_sepcon; apply FF_left).
+rewrite <- H1.
+case_eq (access_mode t2); intros; try (rewrite FF_sepcon; apply FF_left).
+simpl eval_lvalue.
+unfold lift1. unfold_lift. 
+rewrite TE1. rewrite H4; simpl eval_field.
+rewrite field_offset_unroll in H5. rewrite H5.
+normalize.
+(* apply exp_right with v0. *)
+repeat apply andp_right; try apply prop_right; auto.
+hnf; simpl. rewrite TE1.
+rewrite H5. rewrite tc_andp_TT2.
+rewrite denote_tc_assert_andp.
+split; auto. rewrite H7; auto.
+apply sepcon_derives; auto.
+simpl.
+apply orp_right2. apply andp_right; try apply prop_right; auto.
+apply exp_right with v0; auto.
+repeat apply andp_right; try apply prop_right; auto.
+hnf; simpl. hnf in H3. simpl in H3.
+rewrite denote_tc_assert_andp in H3. destruct H3.
+eapply expr_lemmas.typecheck_val_eval_cast; eassumption.
+
+intros ek vl rho; unfold local, lift1; unfold_lift; unfold normal_ret_assert; simpl.
+unfold_lift.
+normalize.
+apply sepcon_derives; auto.
+unfold mapsto, umapsto, field_mapsto.
+rewrite TE1.
+case_eq (access_mode t2); intros; normalize.
+unfold eval_field.
+rewrite field_offset_unroll.
+unfold offset_val, always.
+case_eq (field_offset fld fields); intros; normalize.
+case_eq (eval_lvalue e1 rho); intros; normalize.
+rewrite <- H1. rewrite H4.
+normalize.
+apply orp_left; auto.
+normalize.
+rewrite H7 in H2; inv H2.
+Opaque field_mapsto.
+Qed.
+
+Lemma semax_store_field_mapsto: 
+forall Espec (Delta: tycontext) sh e1 fld P v0 t2 e2 sid fields ,
+    writable_share sh ->
+    typeof e1 = Tstruct sid fields noattr ->
+    t2 = type_of_field
+             (unroll_composite_fields sid (Tstruct sid fields noattr) fields) fld ->
+    typecheck_store (Efield e1 fld t2) ->
+   @semax Espec Delta 
+       (|> (local (tc_lvalue Delta e1) && local (tc_expr Delta (Ecast e2 t2)) &&
+          (`(field_mapsto sh (typeof e1) fld) (eval_lvalue e1) v0 * P)))
+       (Sassign (Efield e1 fld t2) e2) 
+       (normal_ret_assert 
+          (`(field_mapsto sh (typeof e1) fld) (eval_lvalue e1) 
+                  (`(eval_cast (typeof e2) t2) (eval_expr e2)) * P)).
+Proof.
+intros.
+eapply semax_pre0; [ | eapply semax_store_field; eassumption].
+apply later_derives.
+apply andp_derives; auto.
+intro rho; simpl.
+apply sepcon_derives; auto.
+unfold lift.
+unfold_lift. apply field_mapsto_field_mapsto_.
+Qed.
+
+Lemma semax_load_field'':
+forall Espec (Delta: tycontext) n sh id t1 fld P Q R e1 v1 v2 t2 i2 sid fields ,
+    t1 = Tstruct sid fields noattr ->
+    typeof e1 = t1 ->
+        (temp_types Delta) ! id = Some (t2,i2) ->
+   t2 = type_of_field
+             (unroll_composite_fields sid (Tstruct sid fields noattr) fields) fld ->
+     Cop.classify_cast t2 t2 = Cop.cast_case_neutral ->
+     PROPx P (LOCALx (tc_environ Delta :: Q) (SEPx R)) |-- local (tc_lvalue Delta e1) ->
+    PROPx P (LOCALx (tc_environ Delta :: Q) (SEPx R)) |-- local (`eq v1 (eval_lvalue e1)) ->
+    nth_error R n = Some (`(field_mapsto sh t1 fld) v1 v2) ->
+    @semax Espec Delta 
+       (|> PROPx P (LOCALx Q (SEPx R)))
+       (Sset id (Efield e1 fld t2))
+       (normal_ret_assert 
+        (EX old:val,
+          PROPx P (LOCALx (`eq (eval_id id) (subst id (`old) v2) :: map (subst id (`old)) Q)
+                (SEPx 
+                  (map (subst id (`old))
+                    (replace_nth n R (`(field_mapsto sh t1 fld) (eval_lvalue e1) v2))))))).
+Proof.
+intros. rename H3 into CC.
+eapply semax_pre_post;
+  [ | |  apply (semax_load_field Espec Delta sh id t1 fld (PROPx P (LOCALx Q (SEPx (replace_nth n R emp)))) e1
+   v2 t2 i2 sid fields)]; auto; try congruence.
+match goal with |- ?P |-- _ => 
+ let P' := strip1_later P in apply derives_trans with (|>P' )
+end.
+rewrite later_andp; apply andp_derives; auto; apply now_later.
+apply later_derives.
+rewrite insert_local.
+rewrite (local_andp_lemma _ _ H4).
+rewrite (local_andp_lemma _ _ H5).
+rewrite <- insert_local.
+assert (PROPx P (LOCALx Q (SEPx R)) |-- local (`isptr v1)).
+clear - H6.
+intro rho; unfold PROPx,LOCALx,SEPx',local,lift1,tc_expr,tc_lvalue; unfold_lift; simpl.
+repeat (apply derives_extract_prop; intro).
+change SEPx with SEPx'.
+ unfold PROPx,LOCALx,SEPx',local,lift1,tc_expr,tc_lvalue; unfold_lift; simpl.
+unfold_lift in H6.
+revert R H6; induction n; destruct R; simpl; intros; inv H6.
+rewrite field_mapsto_isptr. normalize.
+apply derives_trans with (TT * (!!isptr (v1 rho) && TT)).
+apply sepcon_derives; auto. rewrite andp_TT; auto. normalize.
+ rewrite (local_andp_lemma _ _ H3).
+change SEPx with SEPx'.
+intro rho; unfold PROPx,LOCALx,SEPx',local,lift1,tc_expr,tc_lvalue; unfold_lift; simpl.
+repeat (apply derives_extract_prop; intro).
+repeat apply andp_right; try apply prop_right; auto.
+normalize.
+repeat apply andp_right; try apply prop_right; auto.
+rewrite <- H8.
+clear - H6. rename H6 into H5.
+clear - H5; revert R H5; induction n; destruct R; simpl; intros; inv H5.
+rewrite emp_sepcon; apply sepcon_derives; auto.
+rewrite <- sepcon_assoc.
+rewrite (sepcon_comm (field_mapsto _ _ _ _ _)).
+rewrite sepcon_assoc.
+apply sepcon_derives; auto.
+
+intros ek vl rho.
+unfold normal_ret_assert.
+normalize.
+autorewrite with subst.
+normalize.
+apply exp_right with old.
+normalize.
+clear - H6. rename H6 into H5.
+clear - H5; revert R H5; induction n; destruct R; simpl; intros; inv H5.
+apply sepcon_derives. apply derives_refl.
+rewrite closed_wrt_subst by (auto with closed). rewrite emp_sepcon; auto.
+rewrite <- sepcon_assoc.
+rewrite (sepcon_comm (field_mapsto _ _ _ _ _)).
+rewrite sepcon_assoc.
+apply sepcon_derives; auto.
+Qed.
+
+Lemma semax_load_field_deref'':
+forall Espec (Delta: tycontext) n sh id t1 fld P Q R e1 v1 v2 t2 i2 sid fields ,
+    t1 = Tstruct sid fields noattr ->
+    typeof e1 = tptr t1 ->
+        (temp_types Delta) ! id = Some (t2,i2) ->
+   t2 = type_of_field
+             (unroll_composite_fields sid (Tstruct sid fields noattr) fields) fld ->
+     Cop.classify_cast t2 t2 = Cop.cast_case_neutral ->
+     PROPx P (LOCALx (tc_environ Delta :: Q) (SEPx R)) |-- local (tc_expr Delta e1) ->
+    PROPx P (LOCALx (tc_environ Delta :: Q) (SEPx R)) |-- local (`eq v1 (eval_expr e1)) ->
+    nth_error R n = Some (`(field_mapsto sh t1 fld) v1 v2) ->
+    @semax Espec Delta 
+       (|> PROPx P (LOCALx Q (SEPx R)))
+       (Sset id (Efield (Ederef e1 t1) fld t2))
+       (normal_ret_assert 
+        (EX old:val,
+          PROPx P (LOCALx (`eq (eval_id id) (subst id (`old) v2) :: map (subst id (`old)) Q)
+                (SEPx 
+                  (map (subst id (`old))
+                    (replace_nth n R (`(field_mapsto sh t1 fld) (eval_expr e1) v2))))))).
+Proof.
+intros. rename H3 into CC.
+eapply semax_pre_post;
+  [ | |  apply (semax_load_field Espec Delta sh id t1 fld (PROPx P (LOCALx Q (SEPx (replace_nth n R emp)))) (Ederef e1 t1)
+   v2 t2 i2 sid fields)]; auto; try congruence.
+match goal with |- ?P |-- _ => 
+ let P' := strip1_later P in apply derives_trans with (|>P' )
+end.
+rewrite later_andp; apply andp_derives; auto; apply now_later.
+apply later_derives.
+rewrite insert_local.
+rewrite (local_andp_lemma _ _ H4).
+rewrite (local_andp_lemma _ _ H5).
+rewrite <- insert_local.
+assert (PROPx P (LOCALx Q (SEPx R)) |-- local (`isptr v1)).
+clear - H6.
+intro rho; unfold PROPx,LOCALx,SEPx',local,lift1,tc_expr,tc_lvalue; unfold_lift; simpl.
+repeat (apply derives_extract_prop; intro).
+change SEPx with SEPx'.
+ unfold PROPx,LOCALx,SEPx',local,lift1,tc_expr,tc_lvalue; unfold_lift; simpl.
+unfold_lift in H6.
+revert R H6; induction n; destruct R; simpl; intros; inv H6.
+rewrite field_mapsto_isptr. normalize.
+apply derives_trans with (TT * (!!isptr (v1 rho) && TT)).
+apply sepcon_derives; auto. rewrite andp_TT; auto. normalize.
+ rewrite (local_andp_lemma _ _ H3).
+change SEPx with SEPx'.
+intro rho; unfold PROPx,LOCALx,SEPx',local,lift1,tc_expr,tc_lvalue; unfold_lift; simpl.
+repeat (apply derives_extract_prop; intro).
+repeat apply andp_right; try apply prop_right; auto.
+repeat rewrite denote_tc_assert_andp.
+rewrite H0, H. repeat split; simpl; auto.
+unfold_lift; rewrite <- H8; apply H10.
+normalize.
+rewrite <- H8.
+clear - H6. rename H6 into H5.
+clear - H5; revert R H5; induction n; destruct R; simpl; intros; inv H5.
+rewrite emp_sepcon; apply sepcon_derives; auto.
+rewrite <- sepcon_assoc.
+rewrite (sepcon_comm (field_mapsto _ _ _ _ _)).
+rewrite sepcon_assoc.
+apply sepcon_derives; auto.
+
+intros ek vl rho.
+unfold normal_ret_assert.
+normalize.
+autorewrite with subst.
+normalize.
+apply exp_right with old.
+normalize.
+simpl eval_lvalue. autorewrite with subst. normalize.
+clear - H6. rename H6 into H5.
+clear - H5; revert R H5; induction n; destruct R; simpl; intros; inv H5.
+apply sepcon_derives. apply derives_refl.
+rewrite closed_wrt_subst by (auto with closed). rewrite emp_sepcon; auto.
+rewrite <- sepcon_assoc.
+rewrite (sepcon_comm (field_mapsto _ _ _ _ _)).
+rewrite sepcon_assoc.
+apply sepcon_derives; auto.
+Qed.
+
+
+Lemma semax_store_field'':
+forall Espec (Delta: tycontext) n sh t1 fld P Q R e1 v1 e2 t2 sid fields
+    (WS: writable_share sh) ,
+    t1 = Tstruct sid fields noattr ->
+    typeof e1 = t1 ->
+    t2 = type_of_field (unroll_composite_fields sid (Tstruct sid fields noattr) fields) fld ->
+    typecheck_store (Efield e1 fld t2) ->
+     PROPx P (LOCALx (tc_environ Delta :: Q) (SEPx R)) |-- local (tc_lvalue Delta e1) ->
+     PROPx P (LOCALx (tc_environ Delta :: Q) (SEPx R)) |-- local (tc_expr Delta (Ecast e2 t2)) ->
+    PROPx P (LOCALx (tc_environ Delta :: Q) (SEP (TT))) |-- local (`eq v1 (eval_lvalue e1)) ->
+    nth_error R n = Some (`(field_mapsto_ sh t1 fld) v1) ->
+    @semax Espec Delta 
+       (|> PROPx P (LOCALx Q (SEPx R)))
+       (Sassign (Efield e1 fld t2) e2) 
+       (normal_ret_assert
+          (PROPx P (LOCALx Q
+              (SEPx (replace_nth n R
+                    (`(field_mapsto sh t1 fld) v1 (`(eval_cast (typeof e2) t2) (eval_expr e2)))))))).
+Proof.
+intros.
+assert (SF := semax_store_field). unfold_lift.
+unfold_lift in SF.
+subst t1.
+specialize (SF Espec Delta sh e1 fld (PROPx P (LOCALx Q (SEPx (replace_nth n R emp))))
+   t2 e2 sid fields WS H0 H1 H2).
+eapply semax_pre_post; [ | | eapply SF]; try eassumption; clear SF.
+eapply derives_trans; [apply andp_derives; [ apply now_later | apply derives_refl] | ].
+rewrite <- later_andp.
+apply later_derives.
+rewrite insert_local.
+assert (H1': PROPx P (LOCALx (tc_environ Delta :: Q) (SEPx R)) |-- local (`eq v1 (eval_lvalue e1))).
+ {  eapply derives_trans; [ | apply H5].
+  apply andp_derives; auto. apply andp_derives; auto. change SEPx with SEPx'; unfold SEPx'.
+  unfold fold_right at 2. rewrite sepcon_emp. apply TT_right.
+ }
+assert (PROPx P (LOCALx (tc_environ Delta :: Q) (SEPx R)) |-- local (`isptr (eval_lvalue e1))).
+  {clear - H1' H6. rename H1' into H4; rename H6 into H5.
+   rewrite (local_andp_lemma _ _ H4).
+   clear H4.
+   unfold_lift.
+   change SEPx with SEPx'; unfold PROPx,LOCALx,SEPx',local,lift1; intro rho; simpl in *.
+   apply derives_extract_prop; intro. unfold_lift in H. rewrite <- H. clear e1 H.
+   apply andp_left2. apply andp_left2.
+   unfold_lift in H5.
+   revert R H5; induction n; destruct R; intros; inv H5; simpl in *; auto.
+   rewrite field_mapsto__isptr. normalize.
+   apply derives_trans with (TT * (!!isptr (v1 rho) && TT)).
+   apply sepcon_derives; auto. rewrite andp_TT. auto.
+   normalize.
+  }
+rewrite (local_andp_lemma _ _ H1').
+rewrite (local_andp_lemma _ _ H3).
+rewrite (local_andp_lemma _ _ H4).
+change SEPx with SEPx'.
+intro rho; unfold PROPx, LOCALx, SEPx', local, lift1,lift2.
+simpl.
+unfold_lift.
+repeat (apply derives_extract_prop; intro).
+destruct H11.
+unfold tc_lvalue. simpl typecheck_lvalue.
+repeat rewrite prop_true_andp by auto.
+rewrite <- H7. rewrite <- H0 in H6.
+clear - H6. rename H6 into H0.
+revert R H0; induction n; destruct R; simpl; intros; inv H0; auto.
+rewrite emp_sepcon; auto.
+rewrite <- sepcon_assoc.
+rewrite (sepcon_comm (field_mapsto_ _ _ _ _)).
+rewrite sepcon_assoc.
+apply sepcon_derives; auto.
+repeat rewrite denote_tc_assert_andp.
+
+
+intros ek vl rho; unfold normal_ret_assert, local,lift1; unfold_lift; simpl.
+repeat (apply derives_extract_prop; intro).
+repeat apply andp_right; try apply prop_right; auto.
+
+rewrite H0.
+match goal with |- ?A |-- _ => apply derives_trans with (local (`eq v1 (eval_lvalue e1)) rho && A) end.
+apply andp_right; auto.
+eapply derives_trans; [ | apply H5].
+normalize.
+apply andp_right; apply prop_right; auto.
+unfold tc_environ, exit_tycon. subst ek. apply H.
+apply derives_extract_prop; intro. unfold_lift in H9. rewrite <- H9.
+change SEPx with SEPx'; unfold PROPx,LOCALx,SEPx',local,lift1; simpl.
+normalize. simpl.
+clear - H6; revert R H6; induction n; destruct R; simpl; intros; inv  H6.
+rewrite emp_sepcon; auto.
+rewrite <- sepcon_assoc.
+rewrite (sepcon_comm (field_mapsto _ _ _ _ _)).
+rewrite sepcon_assoc.
+apply sepcon_derives; auto.
+Qed.
+
+Lemma semax_store_field_deref'':
+forall Espec (Delta: tycontext) n sh t1 fld P Q R e1 v1 e2 t2 sid fields
+    (WS: writable_share sh) ,
+    t1 = Tstruct sid fields noattr ->
+    typeof e1 = tptr t1 ->
+    t2 = type_of_field (unroll_composite_fields sid (Tstruct sid fields noattr) fields) fld ->
+    typecheck_store (Efield e1 fld t2) ->
+     PROPx P (LOCALx (tc_environ Delta :: Q) (SEPx R)) |-- local (tc_expr Delta e1) ->
+     PROPx P (LOCALx (tc_environ Delta :: Q) (SEPx R)) |-- local (tc_expr Delta (Ecast e2 t2)) ->
+    PROPx P (LOCALx (tc_environ Delta :: Q) (SEP (TT))) |-- local (`eq v1 (eval_expr e1)) ->
+    nth_error R n = Some (`(field_mapsto_ sh t1 fld) v1) ->
+    @semax Espec Delta 
+       (|> PROPx P (LOCALx Q (SEPx R)))
+       (Sassign (Efield (Ederef e1 t1) fld t2) e2) 
+       (normal_ret_assert
+          (PROPx P (LOCALx Q
+              (SEPx (replace_nth n R
+                    (`(field_mapsto sh t1 fld) v1 (`(eval_cast (typeof e2) t2) (eval_expr e2)))))))).
+Proof.
+intros.
+assert (H1': PROPx P (LOCALx (tc_environ Delta :: Q) (SEPx R)) |-- local (`eq v1 (eval_expr e1))).
+ {  eapply derives_trans; [ | apply H5].
+  apply andp_derives; auto. apply andp_derives; auto. change SEPx with SEPx'; unfold SEPx'.
+  unfold fold_right at 2. rewrite sepcon_emp. apply TT_right.
+ }
+match goal with |- semax _ _ _ ?Post => 
+apply semax_pre_post with
+(P':= |>PROPx P (LOCALx (`isptr (eval_expr e1) :: Q) (SEPx R)))
+(R' := Post)
+end.
+eapply derives_trans; [apply andp_derives; [ apply now_later | apply derives_refl] | ].
+rewrite <- later_andp.
+apply later_derives.
+rewrite <- insert_local.
+apply andp_right; auto.
+rewrite insert_local.
+rewrite (local_andp_lemma _ _ H1').
+intro rho.
+simpl.
+rewrite <- insert_local.
+simpl.
+repeat (apply derives_extract_prop; intro).
+unfold_lift in H7.
+normalize.
+rewrite <- H7.
+clear - H6.
+revert R H6; induction n; destruct R; simpl; intros; inv H6.
+normalize. rewrite field_mapsto__isptr; normalize.
+apply derives_trans with (TT * (!!isptr (v1 rho) && TT)).
+apply sepcon_derives; auto. rewrite andp_TT; auto. normalize.
+apply andp_left2; auto.
+intros. apply andp_left2; auto.
+assert (SF := semax_store_field'' Espec Delta n sh t1 fld P (`isptr (eval_expr e1) :: Q) R
+  (Ederef e1 t1) v1 e2 t2 sid fields WS).
+eapply semax_pre_post; [ | | eapply SF]; try eassumption; clear SF; auto.
+apply andp_left2; auto.
+intros; apply andp_left2.
+apply normal_ret_assert_derives'. rewrite <- insert_local. apply andp_left2; auto.
+do 2 rewrite <- insert_local.
+ rewrite <- andp_assoc.
+rewrite (andp_comm (local _) (local _)). rewrite andp_assoc.
+rewrite insert_local. rewrite (local_andp_lemma _ _ H3).
+rewrite <- andp_assoc. 
+apply andp_left1.
+intro rho; unfold local,lift1.
+simpl. rewrite <- prop_and. apply prop_derives.
+unfold tc_lvalue. simpl typecheck_lvalue.
+rewrite H0,H. simpl tc_bool. repeat rewrite tc_andp_TT2.
+rewrite denote_tc_assert_andp. simpl. unfold_lift.
+intros [? ?]; split; auto.
+do 2 rewrite <- insert_local.
+ rewrite <- andp_assoc.
+rewrite (andp_comm (local _) (local _)). rewrite andp_assoc.
+rewrite insert_local. apply andp_left2; auto.
+simpl eval_lvalue.
+do 2 rewrite <- insert_local. rewrite <- andp_assoc.
+rewrite (andp_comm (local _) (local _)). rewrite andp_assoc.
+rewrite insert_local.
+rewrite (local_andp_lemma _ _ H5).
+intro rho.
+simpl.
+repeat (apply derives_extract_prop; intro).
+apply prop_right.
+unfold_lift in H7. unfold_lift in H8. unfold_lift.
+rewrite isptr_force_ptr by auto.
+auto.
+Qed.
+
+(* ALL the rest of the lemmas in this file should (eventually) become obsolete, 
+  in favor of the lemmas earlier in the file  *)
+
+Lemma semax_load_field':
+forall Espec (Delta: tycontext) sh id t1 fld P Q R e1 v2 t2 i2 sid fields ,
+    t1 = Tstruct sid fields noattr ->
+    typeof e1 = t1 ->
+        (temp_types Delta) ! id = Some (t2,i2) ->
+   t2 = type_of_field
+             (unroll_composite_fields sid (Tstruct sid fields noattr) fields) fld ->
+     Cop.classify_cast t2 t2 = Cop.cast_case_neutral ->
+    @semax Espec Delta 
+       (|> PROPx P (LOCALx (tc_lvalue Delta e1::Q) (SEPx (`(field_mapsto sh t1 fld) (eval_lvalue e1) v2::R))))
+       (Sset id (Efield e1 fld t2))
+       (normal_ret_assert 
+        (EX old:val,
+          PROPx P (LOCALx (`eq (eval_id id) (subst id (`old) v2) :: map (subst id (`old)) Q)
+                (SEPx 
+                  (map (subst id (`old))
+                    (`(field_mapsto sh t1 fld) (eval_lvalue e1) v2 :: R)))))).
+Proof.
+intros. rename H3 into CC.
+eapply semax_pre_post;
+  [ | |  apply (semax_load_field Espec Delta sh id t1 fld (PROPx P (LOCALx Q (SEPx R))) e1
+   v2 t2 i2 sid fields)]; auto; try congruence.
+match goal with |- ?P |-- _ => 
+ let P' := strip1_later P in apply derives_trans with (|>P' )
+end.
+rewrite later_andp; apply andp_derives; auto; apply now_later.
+apply later_derives.
+
+change SEPx with SEPx'.
+intro rho; unfold PROPx,LOCALx,SEPx',local,lift1,tc_expr,tc_lvalue; unfold_lift; simpl.
+ rewrite field_mapsto_isptr.
+normalize.
+repeat apply andp_right; try apply prop_right; auto.
+
+intros ek vl rho.
+unfold normal_ret_assert.
+normalize.
+autorewrite with subst.
+try intros old ?. (* Coq 8.3/8.4 compatibility *)
+apply exp_right with old.
+autorewrite with subst. normalize.
+Qed.
+
+
+Lemma semax_load_field_deref:
+forall Espec (Delta: tycontext) sh id t1 fld P Q R e1 v2 t2 i2 sid fields ,
+    t1 = Tstruct sid fields noattr ->
+    typeof e1 = Tpointer t1 noattr ->
+        (temp_types Delta) ! id = Some (t2,i2) ->
+   t2 = type_of_field
+             (unroll_composite_fields sid (Tstruct sid fields noattr) fields) fld ->
+     Cop.classify_cast t2 t2 = Cop.cast_case_neutral ->
+    @semax Espec Delta 
+       (|> PROPx P (LOCALx (tc_expr Delta e1::Q) (SEPx (`(field_mapsto sh t1 fld) (eval_expr e1) v2::R))))
+       (Sset id (Efield (Ederef e1 t1) fld t2))
+       (normal_ret_assert 
+        (EX old:val,
+          PROPx P (LOCALx (`eq (eval_id id) (subst id (`old) v2) :: map (subst id (`old)) Q)
+                (SEPx 
+                  (map (subst id (`old))
+                    (`(field_mapsto sh t1 fld) (eval_expr e1) v2 :: R)))))).
+Proof.
+intros.
+eapply semax_pre_post; [ | | 
+    apply (semax_load_field' Espec Delta sh id t1 fld P Q R (Ederef e1 t1) v2 t2 i2 sid fields); auto].
+eapply derives_trans.
+apply andp_derives. apply now_later. apply derives_refl.
+rewrite <- later_andp. apply later_derives.
+apply go_lower_lem9.
+ change SEPx with SEPx'.
+ intro rho; unfold PROPx, LOCALx, SEPx', local,lift1; unfold_lift.
+simpl.
+apply andp_derives; auto.
+rewrite field_mapsto_isptr.
+rewrite field_mapsto_nonvolatile.
+normalize.
+apply andp_right; auto.
+apply andp_right; apply prop_right; auto.
+hnf; simpl. repeat rewrite denote_tc_assert_andp; repeat split; auto.
+rewrite H0; reflexivity.
+rewrite H8; reflexivity.
+
+intros. apply andp_left2.
+apply normal_ret_assert_derives'.
+apply exp_derives; intro old.
+ change SEPx with SEPx'.
+ intro rho; unfold PROPx, LOCALx, SEPx', local,lift1; unfold_lift.
+simpl.
+apply andp_derives; auto.
+apply andp_derives; auto.
+unfold subst; simpl.
+apply sepcon_derives; auto.
+unfold_lift.
+rewrite field_mapsto_force_ptr.
+auto.
+Qed.
+
+Lemma semax_store_field':
+forall Espec (Delta: tycontext) sh t1 fld P Q R e1 e2 t2 sid fields
+    (WS: writable_share sh) ,
+    t1 = Tstruct sid fields noattr ->
+    typeof e1 = t1 ->
+    t2 = type_of_field (unroll_composite_fields sid (Tstruct sid fields noattr) fields) fld ->
+    typecheck_store (Efield e1 fld t2) ->
+    @semax Espec Delta 
+       (|> PROPx P (LOCALx (tc_lvalue Delta e1::tc_expr Delta (Ecast e2 t2)::Q)
+                             (SEPx (`(field_mapsto_ sh t1 fld) (eval_lvalue e1)::R))))
+       (Sassign (Efield e1 fld t2) e2) 
+       (normal_ret_assert
+          (PROPx P (LOCALx Q
+              (SEPx  (`(field_mapsto sh t1 fld) (eval_lvalue e1) 
+                  (`(eval_cast (typeof e2) t2) (eval_expr e2)) :: R))))).
+Proof.
+intros.
+pose proof semax_store_field. unfold_lift.
+unfold_lift in H3.
+subst t1.
+specialize (H3 Espec Delta sh e1 fld (PROPx P (LOCALx Q (SEPx R)))
+   t2 e2 sid fields WS H0 H1 H2).
+eapply semax_pre_post; [ | | eapply H3]; try eassumption.
+apply andp_left2. apply later_derives.
+change SEPx with SEPx';
+unfold PROPx, LOCALx,SEPx', local,lift1; unfold_lift; intro rho.
+simpl. normalize. rewrite H0; auto. 
+
+intros ek vl rho; unfold normal_ret_assert, local,lift1; unfold_lift; simpl.
+repeat (apply derives_extract_prop; intro); subst.
+repeat apply andp_right; try apply prop_right; auto.
+rewrite H0.
+normalize.
+Qed.
+
+Lemma semax_store_field_deref:
+forall Espec (Delta: tycontext) sh t1 fld P Q R e1 e2 t2 sid fields
+    (WS: writable_share sh) ,
+    t1 = Tstruct sid fields noattr ->
+    typeof e1 = Tpointer t1 noattr ->
+    t2 = type_of_field (unroll_composite_fields sid (Tstruct sid fields noattr) fields) fld ->
+    typecheck_store (Efield (Ederef e1 t1) fld t2) ->
+    @semax Espec Delta 
+       (|> PROPx P (LOCALx (tc_expr Delta e1::tc_expr Delta (Ecast e2 t2)::Q)
+                             (SEPx (`(field_mapsto_ sh t1 fld) (eval_expr e1)::R))))
+       (Sassign (Efield (Ederef e1 t1) fld t2) e2) 
+       (normal_ret_assert
+          (PROPx P (LOCALx Q
+              (SEPx  (`(field_mapsto sh t1 fld) (eval_expr e1) 
+                  (`(eval_cast (typeof e2) t2) (eval_expr e2)) :: R))))).
+Proof.
+intros.
+pose proof (semax_store_field' Espec Delta sh t1 fld P Q R (Ederef e1 t1) e2 t2 sid fields WS H (eq_refl _) H1 H2).
+unfold_lift. unfold_lift in H3.
+eapply semax_pre_post; [  | | eapply H3].
+apply andp_left2; apply later_derives.
+intro rho; simpl; unfold PROPx; simpl; apply andp_derives; auto.
+change SEPx with SEPx'; unfold LOCALx, SEPx'; simpl; normalize.
+
+rewrite field_mapsto__isptr.
+rewrite field_mapsto__nonvolatile.
+simpl; normalize.
+repeat apply andp_right; try apply prop_right; auto.
+hnf; simpl. repeat rewrite denote_tc_assert_andp.
+repeat split; auto. rewrite H0; apply I. rewrite H. apply I.
+
+intros. apply andp_left2; auto.
+apply normal_ret_assert_derives'.
+intro rho; simpl; unfold PROPx; simpl; apply andp_derives; auto.
+change SEPx with SEPx'; unfold LOCALx, SEPx'; simpl; normalize.
+Qed.
+
+Lemma semax_store_PQR:
+forall Espec (Delta: tycontext) sh t1 P Q R e1 e2
+    (WS: writable_share sh)
+    (NONVOL: type_is_volatile t1 = false)
+    (TC: typecheck_store (Ederef e1 t1)),
+    typeof e1 = Tpointer t1 noattr ->
+    @semax Espec Delta 
+       (|> PROPx P (LOCALx (tc_expr Delta e1::tc_expr Delta (Ecast e2 t1)::Q)
+                             (SEPx (`(mapsto_ sh t1) (eval_expr e1)::R))))
+       (Sassign (Ederef e1 t1) e2) 
+       (normal_ret_assert
+          (PROPx P (LOCALx Q
+              (SEPx  (`(mapsto sh t1) (eval_expr e1) 
+                  (`(eval_cast (typeof e2) t1) (eval_expr e2)) :: R))))).
+Proof.
+intros.
+pose proof semax_store.
+unfold_lift; unfold_lift in H0.
+eapply semax_pre_post; [ | | eapply (H0 Delta (Ederef e1 t1) e2 sh)]; try eassumption.
+instantiate (1:=(PROPx P (LOCALx Q (SEPx R)))).
+apply andp_left2. apply later_derives. change SEPx with SEPx'.
+intro rho; unfold PROPx, LOCALx, SEPx', local, lift1,lift2.
+simpl.
+unfold_lift.
+normalize.
+unfold tc_lvalue. simpl typecheck_lvalue.
+rewrite H; simpl.
+rewrite mapsto__isptr at 1. normalize.
+repeat apply andp_right; try apply prop_right; auto.
+repeat rewrite denote_tc_assert_andp.
+repeat split; auto.
+rewrite NONVOL; hnf; unfold_lift; hnf; auto.
+replace (force_ptr (eval_expr e1 rho)) with (eval_expr e1 rho); auto.
+clear - H5; hnf in H5. destruct (eval_expr e1 rho); try contradiction; simpl; auto.
+
+intros ek vl rho; unfold normal_ret_assert, local,lift1; unfold_lift; simpl. unfold_lift.
+repeat (apply derives_extract_prop; intro).
+subst. repeat rewrite prop_true_andp by auto.
+normalize.
+cancel.
+clear.
+rewrite mapsto_isptr at 1. normalize.
+replace (force_ptr (eval_expr e1 rho)) with (eval_expr e1 rho); auto.
+destruct (eval_expr e1 rho); simpl in *; try contradiction; auto.
+Qed.
+
+Lemma semax_load':
+  forall Espec (Delta : tycontext) (sh : Share.t) (id : positive) 
+         P Q R (e1 : expr) t1 i2 (v2 : environ -> val),
+   typeof e1 = Tpointer t1 noattr ->
+   (temp_types Delta) ! id = Some (t1,i2) ->
+   type_is_volatile t1 = false ->
+   classify_cast t1 t1 = cast_case_neutral ->
+ @semax Espec Delta
+     (|> PROPx P (LOCALx (tc_expr Delta e1 ::  Q)
+            (SEPx (`(mapsto sh t1) (eval_expr e1) v2 :: R))))
+    (Sset id (Ederef e1 t1))
+    (normal_ret_assert
+       (EX old: val, 
+        PROPx P (LOCALx (`eq (eval_id id) (subst id (`old) v2) ::
+                         map (subst id (`old)) Q)
+                (SEPx 
+                  (map (subst id (`old))
+                    (`(mapsto sh t1) (eval_expr e1) v2 :: R)))))).
+Proof.
+ intros. rename H2 into CLASSIFY.
+ eapply semax_pre_post;
+  [ | |  apply (semax_load Delta sh id (PROPx P (LOCALx Q (SEPx R))) (Ederef e1 t1)
+   v2)]; auto.
+match goal with |- ?P |-- _ => 
+ let P' := strip1_later P in apply derives_trans with (|>P' )
+end.
+rewrite later_andp; apply andp_derives; auto; apply now_later.
+apply later_derives.
+change SEPx with SEPx'.
+intro rho; unfold PROPx,LOCALx,SEPx',local,lift1,tc_expr,tc_lvalue; unfold_lift; simpl.
+repeat (apply derives_extract_prop; intro).
+rewrite mapsto_isptr.
+rewrite sepcon_andp_prop'.
+apply derives_extract_prop; intro.
+destruct H4.
+rewrite H in *. rewrite H1 in *. simpl.
+unfold mapsto.
+repeat apply andp_right; try apply prop_right; auto.
+repeat rewrite denote_tc_assert_andp.
+repeat split; auto.
+hnf. exists t1, i2. split; auto.
+unfold allowedValCast. rewrite CLASSIFY.
+destruct t1; simpl; auto.
+normalize.
+apply sepcon_derives; auto.
+destruct (eval_expr e1 rho); inv H5; auto.
+
+intros ek vl rho.
+unfold normal_ret_assert.
+normalize. 
+try (intros old ?).  (* Coq 8.3/8.4 compatibility *)
+apply exp_right with old.
+normalize. simpl typeof; unfold eval_lvalue; fold eval_expr.
+autorewrite with subst.
+change SEPx with SEPx'; unfold PROPx,LOCALx,SEPx',local,lift1.
+normalize.
+apply sepcon_derives; auto.
+match goal with |- mapsto _ _ (force_ptr ?E) _ |-- _ =>
+ destruct E; simpl; auto
+end.
+Qed.
+
+
